proof/iu_system/uni/prop_basic.v
@@ -127,7 +127,7 @@ Proof.
       apply notin_singleton_1 in Fr. contradiction.
 Qed.
 
-Lemma lc_typ_subst : forall A1 X T,
+Lemma lc_typ_subst_inv : forall A1 X T,
   lc_typ ({T /ᵈ X} A1) ->
   lc_typ T ->
   lc_typ A1.
@@ -153,6 +153,20 @@ Proof.
     inversion x; eauto.
 Qed.
 
+
+Lemma lc_typ_subst : forall A1 T X,
+  lc_typ A1 ->
+  lc_typ T ->
+  lc_typ ({ T /ᵈ X } A1).
+Proof.
+  intros. induction H; simpl; auto.
+  - destruct (X0 == X); auto.
+  - inst_cofinites_by (singleton X) using_name X. eapply lc_typ_all_exists with (X1:=X0). 
+    replace (({T /ᵈ X} A) ^ᵈ X0) with ({T /ᵈ X} A ^ᵈ X0); eauto.
+    rewrite typ_subst_open_comm; auto.
+Qed.
+
+
 Lemma ftv_sin_typ_subst : forall X Y T1 S1,
   lc_typ S1 ->
   X `notin` ftv_in_typ S1 ->
@@ -176,7 +190,7 @@ Proof.
     + inversion x.
     + apply dsin_arrow1; inversion x; eauto.
       subst.
-      eapply lc_typ_subst; eauto.
+      eapply lc_typ_subst_inv; eauto.
   - destruct T1; simpl; try solve [inversion x].
     simpl in *. destruct (X0 == Y); subst.
     + dependent destruction H.
@@ -185,7 +199,7 @@ Proof.
       contradiction.
     + inversion x.
     + apply dsin_arrow2; inversion x; eauto.
-      subst. eapply lc_typ_subst; eauto.
+      subst. eapply lc_typ_subst_inv; eauto.
   - destruct T1; simpl; try solve [inversion x].
   simpl in *. destruct (X0 == Y); subst.
     + assert (ds_in X (typ_all A)).
@@ -554,11 +568,11 @@ Proof with eauto.
 Qed. *)
 
 
-Lemma d_wft_typ_subst : forall E X F T1 T2,
+Lemma d_wft_typ_subst : forall E X F A1 T2,
   ⊢ F ++ X ~ dbind_tvar_empty ++ E ->
-  F ++ X ~ dbind_tvar_empty ++ E ⊢ T1 ->
+  F ++ X ~ dbind_tvar_empty ++ E ⊢ A1 ->
   E ⊢ T2 ->
-  map (subst_tvar_in_dbind T2 X) F  ++ E ⊢ {T2 /ᵈ X} T1.
+  map (subst_tvar_in_dbind T2 X) F  ++ E ⊢ {T2 /ᵈ X} A1.
 Proof with simpl in *; try solve_by_invert; eauto using uniq_app_1, uniq_app_2.
   intros * Hwfenv Hwft1 Hwft2.
   inductions Hwft1; intros; forwards: d_wf_env_uniq Hwfenv; try solve [simpl; auto]...
@@ -584,11 +598,11 @@ Proof with simpl in *; try solve_by_invert; eauto using uniq_app_1, uniq_app_2.
 Qed.
 
 
-Lemma d_wft_typ_subst_stvar : forall E X F T1 T2,
+Lemma d_wft_typ_subst_stvar : forall E X F A1 T2,
   ⊢ F ++ X ~ dbind_stvar_empty ++ E ->
-  F ++ X ~ dbind_stvar_empty ++ E ⊢ T1 ->
+  F ++ X ~ dbind_stvar_empty ++ E ⊢ A1 ->
   E ⊢ T2 ->
-  map (subst_tvar_in_dbind T2 X) F ++ E ⊢ {T2 /ᵈ X} T1.
+  map (subst_tvar_in_dbind T2 X) F ++ E ⊢ {T2 /ᵈ X} A1.
 Proof with simpl in *; try solve_by_invert; eauto using uniq_app_1, uniq_app_2, binds_app_1, binds_app_2.
   intros * Hwfenv Hwft1 Hwft2.
   inductions Hwft1; intros; forwards: d_wf_env_uniq Hwfenv; try solve [simpl; auto]...
@@ -614,10 +628,10 @@ Proof with simpl in *; try solve_by_invert; eauto using uniq_app_1, uniq_app_2, 
 Qed.
 
 
-Lemma d_new_tv_notin_wf_typ : forall X E T1,
+Lemma d_new_tv_notin_wf_typ : forall X E A1,
   ⊢ (X, dbind_tvar_empty) :: E ->
-  E ⊢ T1 ->
-  X `notin` ftv_in_typ T1.
+  E ⊢ A1 ->
+  X `notin` ftv_in_typ A1.
 Proof.
   intros; induction H0; auto.
   - simpl. destruct (X0 == X).
@@ -640,7 +654,7 @@ Proof.
       rewrite ftv_in_typ_open_typ_wrt_typ_lower; auto.
 Qed.
 
-Lemma dwf_typ_lc_typ : forall E T,
+Lemma d_wf_typ_lc_typ : forall E T,
   E ⊢ T -> lc_typ T.
 Proof.
   intros. induction H; eauto.
@@ -654,23 +668,22 @@ Proof.
   intros; induction H; eauto...
 Qed.
 
-(* bookmark for refactoring *)
 
-Lemma d_neq_all_subst_neq_all : forall T1 X T2,
-  lc_typ T1 ->
-  dmono_typ T2 ->
-  dneq_all T1 ->
-  dneq_all ( {T2 /ᵈ X} T1 ).
+Lemma d_neq_all_subst_neq_all : forall E A1 X T2,
+  lc_typ A1 ->
+  d_mono_typ E T2 ->
+  neq_all A1 ->
+  neq_all ( {T2 /ᵈ X} A1 ).
 Proof.
   intros. induction H; simpl; eauto...
   - destruct (X0 == X); auto.
-    apply d_mono_typ_neq_all; auto.
-  - eapply dneqall_arrow;
+    eapply d_mono_typ_neq_all; eauto.
+  - eapply neq_all__arrow;
     apply subst_tvar_in_typ_lc_typ; eauto...
   - inversion H1.
-  - eapply dneqall_union;
+  - eapply neq_all__union;
     apply subst_tvar_in_typ_lc_typ; eauto...
-  - eapply dneqall_intersection;
+  - eapply neq_all__intersection;
     apply subst_tvar_in_typ_lc_typ; eauto...
 Qed.
 
@@ -679,7 +692,7 @@ Lemma bind_typ_subst : forall F X E x T1 T2,
   ⊢ F ++ (X, dbind_tvar_empty) :: E ->
   x ~ T1 ∈ (F ++ (X, dbind_tvar_empty) :: E) ->
   E ⊢ T2 ->
-  x ~ ({T2 /ᵈ X} T1) ∈ (map (subst_tvar_in_binding T2 X) F ++ E).
+  x ~ ({T2 /ᵈ X} T1) ∈ (map (subst_tvar_in_dbind T2 X) F ++ E).
 Proof.
   intros. induction F; simpl in *; auto.
   - inversion H0.
@@ -696,12 +709,12 @@ Proof.
 Qed.
 
 
-Lemma d_mono_typ_subst_mono_mono : forall T1 T2 X,
-  dmono_typ T1 ->
-  dmono_typ T2 ->
-  dmono_typ ({T2 /ᵈ X} T1).
+Lemma d_mono_typ_subst_mono_mono : forall E A1 T1 X,
+  d_mono_typ E A1 ->
+  d_mono_typ E T1 ->
+  d_mono_typ E ({T1 /ᵈ X} A1).
 Proof.
-  intros. induction T1; try solve [simpl; eauto].
+  intros. induction A1; try solve [simpl; eauto].
   - simpl. destruct (X0 == X); auto.
   - simpl. dependent destruction H. auto.
   - inversion H.
@@ -710,76 +723,76 @@ Proof.
 Qed.
 
 
-Lemma d_sub_dwft : forall E T1 T2,
-  E ⊢ T1 <: T2 -> ⊢ E /\ E ⊢ T1 /\ E ⊢ T2.
+Lemma d_sub_dwft : forall E A1 B1,
+  E ⊢ A1 <: B1 -> ⊢ E /\ E ⊢ A1 /\ E ⊢ B1.
 Proof with auto.
   intros.
   induction H; try solve [intuition].
   - split.
     inst_cofinites_by L. intuition... inversion H3. auto.
-    split; inst_cofinites_for dwftyp_all; intros; inst_cofinites_with X.
-    + eapply fstv_open_tvar; auto.
-    + applys* d_wf_typ_subst_tvar_stvar_cons. auto.
-    + eapply fstv_open_tvar; auto.
-    + applys* d_wf_typ_subst_tvar_stvar_cons. auto.
+    split; eapply d_wf_typ__all with (L:=L `union` ftv_in_typ A1 `union` ftv_in_typ B1); intros; inst_cofinites_with X; auto...
+    eapply d_wf_typ_subst_tvar_stvar_cons; intuition.
+    eapply d_wf_typ_subst_tvar_stvar_cons; intuition.
   - split; try solve [intuition].
     split; try solve [intuition].
-    + eapply dwftyp_all with (L:=L `union` ftv_in_typ S1 `union` dom E).
+    + eapply d_wf_typ__all with (L:=L `union` ftv_in_typ A1 `union` dom E).
       * intros. inst_cofinites_with X. auto.
       * intros. inst_cofinites_with X.
         destruct IHd_sub. auto.
         eapply dwf_typ_open_inv with (X:=X) (S1:=T2); auto.
+        -- eapply d_mono_typ_lc; eauto.
         -- replace (X ~ dbind_tvar_empty ++ E) with (nil ++ X ~ dbind_tvar_empty ++ E) by auto.
            apply dwf_typ_weakening. simpl. rewrite  subst_tvar_in_typ_open_typ_wrt_typ.
            ++ simpl. unfold eq_dec. destruct ( EqDec_eq_of_X X X ).
               ** rewrite subst_tvar_in_typ_fresh_eq; intuition.
               ** contradiction.
-           ++ eapply dwf_typ_dlc_type; eauto.
+           ++ eapply d_mono_typ_lc; eauto.
            (* ++ auto. *)
 Qed.
 
-Lemma d_sub_dwft_0 : forall E T1 T2,
-    E ⊢ T1 <: T2 -> ⊢ E.
-Proof.
-  intros. forwards*: d_sub_dwft H.
-Qed.
-Lemma d_sub_dwft_1 : forall E T1 T2,
-    E ⊢ T1 <: T2 -> E ⊢ T1.
-Proof.
-  intros. forwards*: d_sub_dwft H.
-Qed.
-Lemma d_sub_dwft_2 : forall E T1 T2,
-    E ⊢ T1 <: T2 -> E ⊢ T2.
+Lemma d_sub_dwft_0 : forall E A1 B1,
+    E ⊢ A1 <: B1 -> ⊢ E.
 Proof.
   intros. forwards*: d_sub_dwft H.
 Qed.
 
-Lemma dwf_typ_strengthening : forall F E x T b,
-    ⊢ E ++ x ~ b ++ F ->
-    E ++ x ~ b ++ F ⊢ T ->
-    x \notin ftv_in_typ T ->
-    x \notin fstv_in_typ T ->
+Lemma d_sub_dwft_1 : forall E A1 B1,
+    E ⊢ A1 <: B1 -> E ⊢ A1.
+Proof.
+  intros. forwards*: d_sub_dwft H.
+Qed.
+
+Lemma d_sub_dwft_2 : forall E A1 B1,
+    E ⊢ A1 <: B1 -> E ⊢ B1.
+Proof.
+  intros. forwards*: d_sub_dwft H.
+Qed.
+
+Lemma dwf_typ_strengthening : forall F E X T b,
+    ⊢ E ++ X ~ b ++ F ->
+    E ++ X ~ b ++ F ⊢ T ->
+    X \notin ftv_in_typ T ->
     E ++ F ⊢ T.
 Proof with eauto.
   intros * Hwfenv H. intros.
   dependent induction H; auto.
   - induction E.
-    + inversion H. dependent destruction H2.
+    + inversion H. dependent destruction H1.
       simpl in H0. apply notin_singleton_1 in H0. contradiction.
       auto.
     + destruct a. inversion H.
-      * dependent destruction H2. auto.
+      * dependent destruction H1. auto.
       * simpl. apply dwf_typ_weakening_cons. apply IHE; auto.
-        rewrite_env ((a, b0) :: (E ++ x ~ b ++ F)) in Hwfenv. applys* d_wf_env_strenthening_head.
+        rewrite_env ((a, d) :: (E ++ X ~ b ++ F)) in Hwfenv. applys* d_wf_env_strenthening_head.
         (* forwards: d_wf_env_uniq Hwfenv. solve_uniq. *)
   - induction E.
-    + inversion H. dependent destruction H2.
-      * simpl in H1. apply notin_singleton_1 in H1. contradiction.
+    + inversion H. dependent destruction H1.
+      * simpl in H0. apply notin_singleton_1 in H0. contradiction.
       * auto.
     + destruct a. inversion H.
-      * dependent destruction H2. auto.
+      * dependent destruction H1. auto.
       * simpl. apply dwf_typ_weakening_cons; auto. apply IHE; auto.
-        rewrite_env ((a, b0) :: (E ++ x ~ b ++ F)) in Hwfenv. applys* d_wf_env_strenthening_head.
+        rewrite_env ((a, d) :: (E ++ X ~ b ++ F)) in Hwfenv. applys* d_wf_env_strenthening_head.
         (* forwards: d_wf_env_uniq Hwfenv. solve_uniq. *)
   - simpl in *. constructor.
     + apply notin_union_1 in H1.
@@ -787,12 +800,11 @@ Proof with eauto.
     + apply notin_union_2 in H1.
       eauto.
   - simpl in *.
-    apply dwftyp_all with (L:=L `union` singleton x `union` dom E `union` dom F); intros; inst_cofinites_with X.
+    apply d_wf_typ__all with (L:=L `union` singleton X `union` dom E `union` dom F); intros; inst_cofinites_with X0.
     + auto.
-    + replace (X ~ dbind_tvar_empty ++ E ++ F) with ((X ~ dbind_tvar_empty ++ E)++ F) by auto. eapply H1 with (x:=x) (b:=b); auto.
-      * rewrite_env (X ~ dbind_tvar_empty ++ (E ++ (x, b) :: F)). econstructor...
+    + replace (X0 ~ dbind_tvar_empty ++ E ++ F) with ((X0 ~ dbind_tvar_empty ++ E)++ F) by auto. eapply H1 with (X:=X) (b:=b); auto.
+      * rewrite_env (X0 ~ dbind_tvar_empty ++ (E ++ (X, b) :: F)). econstructor...
       * rewrite ftv_in_typ_open_typ_wrt_typ_upper; auto.
-      * rewrite fstv_in_typ_open_typ_wrt_typ_upper; auto.
   - simpl in *. eauto.
   - simpl in *. eauto.
 Qed.
@@ -801,249 +813,249 @@ Qed.
 Lemma d_wf_env_subst_tvar_typ : forall E X F T1,
   ⊢ F ++ X ~ dbind_tvar_empty ++ E ->
   E ⊢ T1 ->
-  ⊢ (map (subst_tvar_in_binding T1 X) F ++ E).
+  ⊢ (map (subst_tvar_in_dbind T1 X) F ++ E).
 Proof with eauto using d_wft_typ_subst.
   intros * HE HT.
   induction F; intros; simpl.
   - inverts~ HE.
-  - destruct a. rewrite_env ((a, b) :: (F ++ X ~ dbind_tvar_empty ++ E)) in HE.
+  - destruct a. rewrite_env ((a, d) :: (F ++ X ~ dbind_tvar_empty ++ E)) in HE.
     forwards HE': d_wf_env_strenthening_head HE.
     forwards~ IH: IHF.
-    rewrite_env ([(a, subst_tvar_in_binding T1 X b)]
-                   ++ (map (subst_tvar_in_binding T1 X) F ++ E)).
+    rewrite_env ([(a, subst_tvar_in_dbind T1 X d)]
+                   ++ (map (subst_tvar_in_dbind T1 X) F ++ E)).
     forwards: d_wf_env_uniq HE.
-    inverts H. destruct b...
+    inverts H. destruct d...
     + econstructor...
       applys d_wft_typ_subst...
       inverts~ HE.
 Qed.
 
 (* This lemma cannot be used for svar subst because E ⊢ SY does not hold when SY is not in E *)
-Lemma d_wf_env_subst_stvar_typ : forall E SX F T1,
-  ⊢ F ++ SX ~ dbind_stvar_empty ++ E ->
+Lemma d_wf_env_subst_stvar_typ : forall E X F T1,
+  ⊢ F ++ X ~ dbind_stvar_empty ++ E ->
   E ⊢ T1 ->
-  ⊢ (map (d_subst_stv_in_binding T1 SX) F ++ E).
-Proof with eauto using d_wft_typ_subst_stvar.
+  ⊢ (map (subst_tvar_in_dbind T1 X) F ++ E).
+Proof with eauto using d_wft_typ_subst.
   intros * HE HT.
   induction F; intros; simpl.
   - inverts~ HE.
-  - destruct a. rewrite_env ((a, b) :: (F ++ SX ~ dbind_stvar_empty ++ E)) in HE.
+  - destruct a. rewrite_env ((a, d) :: (F ++ X ~ dbind_stvar_empty ++ E)) in HE.
     forwards HE': d_wf_env_strenthening_head HE.
     forwards~ IH: IHF.
-    rewrite_env ([(a, d_subst_stv_in_binding T1 SX b)]
-                   ++ (map (d_subst_stv_in_binding T1 SX) F ++ E)).
+    rewrite_env ([(a, subst_tvar_in_dbind T1 X d)]
+                   ++ (map (subst_tvar_in_dbind T1 X) F ++ E)).
     forwards: d_wf_env_uniq HE.
-    inverts H. destruct b...
+    inverts H. destruct d...
     + econstructor...
       applys d_wft_typ_subst_stvar...
       inverts~ HE.
 Qed.
 
+(* bookmark for refactoring *)
 
-Corollary d_wf_env_weaken_tvar : forall E1 E2 SX,
+Corollary d_wf_env_weaken_tvar : forall E1 E2 X,
   ⊢ E2 ++ E1 ->
-  SX ∉ dom (E2 ++ E1) ->
-  ⊢ E2 ++ SX ~ ▫ ++ E1.
+  X ∉ dom (E2 ++ E1) ->
+  ⊢ E2 ++ X ~ ▫ ++ E1.
 Proof with eauto.
   intros * HE HT. induction E2; intros.
   - econstructor...
-  - rewrite_env (a :: (E2 ++ SX ~ ▫ ++ E1)). destruct a. destruct b.
+  - rewrite_env (a :: (E2 ++ X ~ ▫ ++ E1)). destruct a. destruct d.
     1: rewrite_env ((a, ▫) :: (E2 ++ E1)) in HE.
     2: rewrite_env ((a, ▪) :: (E2 ++ E1)) in HE.
-    3: rewrite_env ((a, dbind_typ T) :: (E2 ++ E1)) in HE.
+    3: rewrite_env ((a, dbind_typ A) :: (E2 ++ E1)) in HE.
     all: forwards HE': d_wf_env_strenthening_head HE; inverts HE.
     all: econstructor; try solve_notin.
     applys dwf_typ_weakening...
 Qed.
 
-Corollary d_wf_env_weaken_stvar : forall E1 E2 SX,
+Corollary d_wf_env_weaken_stvar : forall E1 E2 X,
   ⊢ E2 ++ E1 ->
-  SX ∉ dom (E2 ++ E1) ->
-  ⊢ E2 ++ SX ~ ▪ ++ E1.
+  X ∉ dom (E2 ++ E1) ->
+  ⊢ E2 ++ X ~ ▪ ++ E1.
 Proof with eauto.
   intros * HE HT. induction E2; intros.
   - econstructor...
-  - rewrite_env (a :: (E2 ++ SX ~ ▪ ++ E1)). destruct a. destruct b.
+  - rewrite_env (a :: (E2 ++ X ~ ▪ ++ E1)). destruct a. destruct d.
     1: rewrite_env ((a, ▫) :: (E2 ++ E1)) in HE.
     2: rewrite_env ((a, ▪) :: (E2 ++ E1)) in HE.
-    3: rewrite_env ((a, dbind_typ T) :: (E2 ++ E1)) in HE.
+    3: rewrite_env ((a, dbind_typ A) :: (E2 ++ E1)) in HE.
     all: forwards HE': d_wf_env_strenthening_head HE; inverts HE.
     all: econstructor; try solve_notin.
     applys dwf_typ_weakening...
 Qed.
 
-Lemma subst_same_stvar_typ_id : forall SX T,
-    {typ_svar SX /ₛᵈ SX} T = T.
+Lemma subst_same_tvar_typ_id : forall X T,
+    {typ_var_f X /ᵈ X} T = T.
 Proof with (try progress case_if); subst; simpl; eauto.
   intros. induction T; simpl...
   all: try rewrite IHT; try rewrite IHT1; try rewrite IHT2...
 Qed.
 
-Lemma subst_same_stvar_binding_id : forall SX a,
-    d_subst_stv_in_binding (typ_svar SX) SX a = a.
-Proof with subst; try rewrite subst_same_stvar_typ_id; simpl; eauto.
+Lemma subst_same_stvar_binding_id : forall X a,
+    subst_tvar_in_dbind (typ_var_f X) X a = a.
+Proof with subst; try rewrite subst_same_tvar_typ_id; simpl; eauto.
   intros. destruct a...
-  induction* T...
+  induction* A...
 Qed.
 
-Lemma subst_same_stvar_map_id : forall SX F,
-    map (d_subst_stv_in_binding (typ_svar SX) SX) F = F.
-Proof with subst; try rewrite subst_same_stvar_typ_id; simpl; eauto.
+Lemma subst_same_tvar_map_id : forall X F,
+    map (subst_tvar_in_dbind (typ_var_f X) X) F = F.
+Proof with subst; try rewrite subst_same_tvar_typ_id; simpl; eauto.
   intros. induction F... destruct a...
   rewrite subst_same_stvar_binding_id. rewrite* IHF.
 Qed.
 
 Lemma dom_subst_id : forall T SX F,
-    dom (map (d_subst_stv_in_binding T SX) F) = dom F.
+    dom (map (subst_tvar_in_dbind T SX) F) = dom F.
 Proof with simpl; eauto.
   intros *. induction* F.
-  - destruct a. destruct b...
+  - destruct a. destruct d...
     all: rewrite IHF...
 Qed.
 
-Lemma d_wf_typ_rename_stvar : forall E F SX T SY,
-  E ++ SX ~ ▪ ++ F  ⊢ T  ->
-  map (d_subst_stv_in_binding (typ_svar SY) SX ) E ++ SY ~ ▪ ++ F ⊢ { typ_svar SY /ₛᵈ SX } T.
+Lemma d_wf_typ_rename_stvar : forall E F X Y A1,
+  E ++ X ~ ▪ ++ F  ⊢ A1  ->
+  map (subst_tvar_in_dbind (typ_var_f Y) X ) E ++ Y ~ ▪ ++ F ⊢ { typ_var_f Y /ᵈ X } A1.
 Proof with try solve_notin; simpl in *; eauto.
   intros * HT.
-  case_eq (SX==SY); intros.
-  1: { subst. rewrite* subst_same_stvar_map_id. rewrite subst_same_stvar_typ_id... }
+  case_eq (X==Y); intros.
+  1: { subst. rewrite* subst_same_tvar_map_id. rewrite subst_same_tvar_typ_id... }
   clear H.
   inductions HT...
-  - econstructor. induction E...
+  - case_if... induction E...
     all: inverts H; try solve_by_invert...
-    + remember (let (x, a0) := a in (x, d_subst_stv_in_binding (typ_svar SY) SX a0)).
-      remember (map (d_subst_stv_in_binding (typ_svar SY) SX) E ++ (SY, ▪) :: F).
-      destruct p. applys binds_cons_3.
+    + remember (let (x, a0) := a in (x, subst_tvar_in_dbind (typ_var_f Y) X a0)).
+      remember (map (subst_tvar_in_dbind (typ_var_f Y) X) E ++ (Y, ▪) :: F).
+      destruct p. 
+      apply dwf_typ_weakening_cons.
       applys IHE...
   - case_if... induction E...
-    + econstructor. case_eq (SX0==SY); intros; subst...
+    + eapply d_wf_typ__stvar. case_eq (X0==Y); intros; subst...
       inverts* H. exfalso. applys C. inverts~ H1.
     + destruct a. inverts H.
       * inverts H0...
       * forwards: IHE...
-        remember (map (d_subst_stv_in_binding (typ_svar SY) SX) E ++ (SY, ▪) :: F).
-        rewrite_env ([(a, d_subst_stv_in_binding (typ_svar SY) SX b)] ++ l).
+        remember (map (subst_tvar_in_dbind (typ_var_f Y) X) E ++ (Y, ▪) :: F).
+        rewrite_env ([(a, subst_tvar_in_dbind (typ_var_f Y) X d)] ++ l).
         applys* dwf_typ_weaken_head.
-  - econstructor; intros; inst_cofinites_with X.
-    + forwards: fstv_sins_typ_subst_stv SX (typ_svar SY) H...
-      replace (typ_var_f X) with ({typ_svar SY /ₛᵈ SX} (typ_var_f X)) in *.
-      rewrite* <- d_subst_stv_in_typ_open_typ_wrt_typ...
-      simpl...
+  - eapply d_wf_typ__all with (L:=L `union` singleton X); intros; inst_cofinites_with X0.
+    + rewrite typ_subst_open_comm; eauto.
+      apply ftv_sin_typ_subst_inv; auto.
     + intros.
-      rewrite d_subst_stv_in_typ_open_comm.
-      forwards: H1 ((X, ▫) :: E)...
-      econstructor. solve_notin.
+      rewrite typ_subst_open_comm; eauto.
+      rewrite_env (map (subst_tvar_in_dbind `ᵈ Y X) (X0 ~ ▫ ++ E) ++ (Y, ▪) :: F).
+      auto.
 Qed.
 
 
-Corollary d_wf_env_rename_stvar : forall E SX F SY,
-  ⊢ F ++ SX ~ dbind_stvar_empty ++ E ->
-  SY ∉ dom (F ++ E) ->
-  ⊢ map (d_subst_stv_in_binding (typ_svar SY) SX) F ++ SY ~ dbind_stvar_empty ++ E.
+Corollary d_wf_env_rename_stvar : forall E X F Y,
+  ⊢ F ++ X ~ dbind_stvar_empty ++ E ->
+  Y ∉ dom (F ++ E) ->
+  ⊢ map (subst_tvar_in_dbind (typ_var_f Y) X) F ++ Y ~ dbind_stvar_empty ++ E.
 Proof with try solve_notin; simpl; eauto.
   intros * HE HT.
-  case_eq (SY == SX); intros.
-  1: { subst. rewrite* subst_same_stvar_map_id. } clear H.
-  rewrite_env ((F ++ SX ~ ▪) ++ E) in HE.
-  forwards HE': d_wf_env_weaken_stvar SY HE. { solve_notin. }
+  case_eq (Y == X); intros.
+  1: { subst. rewrite* subst_same_tvar_map_id. } clear H.
+  rewrite_env ((F ++ X ~ ▪) ++ E) in HE.
+  forwards HE': d_wf_env_weaken_stvar Y HE. { solve_notin. }
   induction F; intros; simpl.
   - inverts~ HE. econstructor...
-  - destruct a. destruct b...
-    + rewrite_env (((a, ▫) :: (F ++ SX ~ ▪) ++ E)) in HE. inverts~ HE.
-      rewrite_env ((a, ▫) :: (F ++ SX ~ ▪) ++ (SY, ▪) :: E) in HE'. inverts~ HE'.
+  - destruct a. destruct d...
+    + rewrite_env (((a, ▫) :: (F ++ X ~ ▪) ++ E)) in HE. inverts~ HE.
+      rewrite_env ((a, ▫) :: (F ++ X ~ ▪) ++ (Y, ▪) :: E) in HE'. inverts~ HE'.
       econstructor...
-    + rewrite_env (((a, ▪) :: (F ++ SX ~ ▪) ++ E)) in HE. inverts~ HE.
-      rewrite_env ((a, ▪) :: (F ++ SX ~ ▪) ++ (SY, ▪) :: E) in HE'. inverts~ HE'.
+    + rewrite_env (((a, ▪) :: (F ++ X ~ ▪) ++ E)) in HE. inverts~ HE.
+      rewrite_env ((a, ▪) :: (F ++ X ~ ▪) ++ (Y, ▪) :: E) in HE'. inverts~ HE'.
       econstructor...
-    + rewrite_env (((a, dbind_typ T) :: (F ++ SX ~ ▪) ++ E)) in HE. inverts~ HE.
-      rewrite_env ((a, dbind_typ T) :: (F ++ SX ~ ▪) ++ (SY, ▪) :: E) in HE'. inverts~ HE'.
+    + rewrite_env (((a, dbind_typ A) :: (F ++ X ~ ▪) ++ E)) in HE. inverts~ HE.
+      rewrite_env ((a, dbind_typ A) :: (F ++ X ~ ▪) ++ (Y, ▪) :: E) in HE'. inverts~ HE'.
       econstructor...
       forwards*: IHF. solve_notin.
       applys d_wf_typ_rename_stvar...
-      rewrite_env ((F ++ SX ~ ▪) ++ E)...
+      rewrite_env ((F ++ X ~ ▪) ++ E)...
 Qed.
-Lemma d_neq_all_rename: forall T SX SY,
-  lc_typ T ->
-  dneq_all T ->
-  dneq_all ({typ_svar SY /ₛᵈ SX} T).
-Proof with  simpl; eauto using dsubst_stv_lc_typ; try solve_by_invert.
-  intros. destruct T...
+
+Lemma d_neq_all_rename: forall A1 X Y,
+  lc_typ A1 ->
+  neq_all A1 ->
+  neq_all ({typ_var_f Y /ᵈ X} A1).
+Proof with  simpl; eauto using lc_typ_subst; try solve_by_invert.
+  intros. destruct A1...
   - case_if; subst*.
-  - eapply dneqall_arrow;
-      applys dsubst_stv_lc_typ...
+  - eapply neq_all__arrow;
+      applys lc_typ_subst...
     all: inverts~ H.
-  - econstructor; applys dsubst_stv_lc_typ; try inverts~ H...
-  - econstructor; applys dsubst_stv_lc_typ; try inverts~ H...
+  - econstructor; applys lc_typ_subst; try inverts~ H...
+  - econstructor; applys lc_typ_subst; try inverts~ H...
 Qed.
 
-Lemma d_neq_intersection_rename: forall T SX SY,
-  lc_typ T ->
-  dneq_intersection T ->
-  dneq_intersection ({typ_svar SY /ₛᵈ SX} T).
-Proof with  simpl; eauto using dsubst_stv_lc_typ; try solve_by_invert.
-  intros. destruct T...
+Lemma d_neq_intersection_rename: forall A1 X Y,
+  lc_typ A1 ->
+  neq_intersection A1 ->
+  neq_intersection ({typ_var_f Y /ᵈ X} A1).
+Proof with  simpl; eauto using lc_typ_subst; try solve_by_invert.
+  intros. destruct A1...
   - case_if; subst*.
-  - eapply dneqintersection_arrow;
-      applys dsubst_stv_lc_typ...
-    all: inverts~ H.
-  - econstructor.
-    forwards*: dsubst_stv_lc_typ SX (typ_all T) (typ_svar SY).
-  - econstructor; applys dsubst_stv_lc_typ; try inverts~ H...
-Qed.
-
-
-Lemma d_neq_union_rename: forall T SX SY,
-  lc_typ T ->
-  dneq_union T ->
-  dneq_union ({typ_svar SY /ₛᵈ SX} T).
-Proof with  simpl; eauto using dsubst_stv_lc_typ; try solve_by_invert.
-  intros. destruct T...
-  - case_if; subst*.
-  - eapply dnequnion_arrow;
-      applys dsubst_stv_lc_typ...
+  - eapply neq_intersection__arrow;
+      applys lc_typ_subst...
     all: inverts~ H.
   - econstructor.
-    forwards*: dsubst_stv_lc_typ SX (typ_all T) (typ_svar SY).
-  - econstructor; applys dsubst_stv_lc_typ; try inverts~ H...
+    forwards*: lc_typ_subst (typ_all A1) (typ_var_f Y) X.
+  - econstructor; applys lc_typ_subst; try inverts~ H...
 Qed.
 
-Lemma rename_mono_typ : forall T SX SY,
+
+Lemma d_neq_union_rename: forall A1 X Y,
+  lc_typ A1 ->
+  neq_union A1 ->
+  neq_union ({typ_var_f Y /ᵈ X} A1).
+Proof with  simpl; eauto using lc_typ_subst; try solve_by_invert.
+  intros. destruct A1...
+  - case_if; subst*.
+  - eapply neq_union__arrow;
+      applys lc_typ_subst...
+    all: inverts~ H.
+  - econstructor.
+    forwards*: lc_typ_subst (typ_all A1) (typ_var_f Y) X.
+  - econstructor; applys lc_typ_subst; try inverts~ H...
+Qed.
+
+(* Lemma rename_mono_typ : forall T SX SY,
     dmono_typ T ->
     {typ_svar SY /ₛᵈ SX} T = T.
 Proof with simpl in *; eauto.
   intros * HM.
   induction HM...
   all: try rewrite IHHM1; try rewrite IHHM2...
-Qed.
+Qed. *)
 
-#[export] Hint Resolve d_neq_all_rename d_neq_intersection_rename d_neq_union_rename rename_mono_typ : sub.
+#[export] Hint Resolve d_neq_all_rename d_neq_intersection_rename d_neq_union_rename : sub.
 
 
-Lemma dneq_all_lc_typ : forall T,
-  dneq_all T -> lc_typ T.
+Lemma neq_all_lc_typ : forall T,
+  neq_all T -> lc_typ T.
 Proof.
   intros. induction H; eauto.
 Qed.
 
 Lemma dneq_intersection_lc_typ : forall T,
-  dneq_intersection T -> lc_typ T.
+  neq_intersection T -> lc_typ T.
 Proof.
   intros. induction H; eauto.
 Qed.
-
 
 Lemma dneq_union_lc_typ : forall T,
-  dneq_union T -> lc_typ T.
+  neq_union T -> lc_typ T.
 Proof.
   intros. induction H; eauto.
 Qed.
 
-#[export] Hint Immediate dneq_all_lc_typ dneq_intersection_lc_typ dneq_union_lc_typ : core.
+#[export] Hint Immediate neq_all_lc_typ dneq_intersection_lc_typ dneq_union_lc_typ : core.
 
 
-Lemma lc_typ_open_stvar_subst_mono : forall S T SY,
-    lc_typ (S ^^ᵈ T) -> dmono_typ T -> lc_typ (S ^ᵈ SY).
+(* Lemma lc_typ_open_stvar_subst_mono : forall S T SY,
+    lc_typ (S ^^ᵈ T) -> d_mono_typ T -> lc_typ (S ^ᵈ SY).
 Proof with try solve_notin; try solve_by_invert; simpl in *; eauto.
   intros * HD HM.
   inductions HD.
@@ -1076,8 +1088,9 @@ Proof with try solve_notin; try solve_by_invert; simpl in *; eauto using lc_typ_
                   forwards*: IHHD2 (typ_var_b 0) T4].
 Qed.
 
-Lemma d_wf_typ_open_stvar_subst_mono : forall E F S T SY,
-    E ++ F ⊢ S ^^ᵈ T -> dmono_typ T -> SY ∉ (dom F)
+
+Lemma d_wf_typ_open_stvar_subst_mono : forall E F S T SY, 
+    E ++ F ⊢ S ^^ᵈ T -> d_mono_typ (E ++ F) T -> SY ∉ (dom F)
     -> E ++ SY ~ ▫ ++ F ⊢ S ^ᵈ SY.
 Proof with try solve_notin; simpl in *; eauto.
   intros * HT HD HN.
@@ -1121,4 +1134,6 @@ Proof with try solve_notin; simpl in *; eauto.
                                  forwards*: H1 SZ ((SZ, ▫) :: E) F HE
       end) ]
       ].
-Qed.
+Qed. 
+
+*)
